#+TITLE: Supplementary Material \\ \small{Heterogenous firing responses leads to diverse coupling to presynaptic activity in a simplified morphological model of layer V pyramidal neurons}
#+AUTHOR: Y. Zerlaut \& A. Destexhe

\newpage

* Derivation of the mean membrane potential solution
<<sec:mean-coeff>>

Equation for $\mu_v(X)$:

\begin{equation}
\left\{
\begin{split}
& \frac{\partial^2 \mu_v}{\partial X^2} = \mu_v(X)-v_0^p \quad \forall X \in [0,L_p] \\
&\frac{\partial^2 \mu_v}{\partial X^2} = \mu_v(X)-v_0^d \quad \forall X \in [L_p,L]  \\
&\frac{\partial \mu_v}{\partial X}|_{X=0} = \gamma^p \, 
\Big( \mu_v(0) - V_0  \Big) \\
&\mu_v(X \rightarrow L_p^-) = \mu_v(X \rightarrow L_p^+) \\
&\frac{\partial \mu_v}{\partial X}_{X \rightarrow L_p^-} = \frac{\lambda^p}{\lambda^d}
\frac{\partial \mu_v}{\partial X}_{X \rightarrow L_p^+} \\
&\frac{\partial \mu_v}{\partial X}_{X=L} = 0 
\end{split}
\right.
\end{equation}

We write the solution on the form:

\begin{equation}
\left\{
\begin{split}
& \mu_v(X) = v_0^p + A \, \cosh(X) + C \, \sinh(X) \quad \forall \, X \in [0,L_p] \\
& \mu_v(X) = v_0^d + B \, \cosh(X-L) + D \, \sinh(X-L) \quad \forall \, X \in [L_pL]
\end{split}
\right.
\end{equation}


- Sealed-end boundary condition at cable end implies $D=0$

- Somatic boudary condition imply: $C = \gamma^p \, (v_0^p - V_0 + A)$

- Then v continuity imply :
    \( v_0^p + A \, \cosh(L_p) +  \gamma^p \, (v_0^p - V_0 + A) \, \sinh(L_p) = v_0^d + B \, \cosh(L_p-L) \)

- Then current conservation imply: 
    \( A \, \sinh(L_p) +  \gamma^p \, (v_0^p - V_0 + A) \, \cosh(L_p) = \frac{\lambda^p}{\lambda^d} \, B \, \sinh(L_p-L) \)

We rewrite those condition on a matrix form:

\begin{equation}
\Big(
\begin{matrix}
    \cosh(L_p)+\gamma^p \sinh(L_p) & -\cosh(L_p-L) \\
    \sinh(L_p)+\gamma^p \cosh(L_p) & -  \frac{\lambda^p}{\lambda^d} \, \sinh(L_p-L) 
\end{matrix}
\Big)
\cdot
\Big(
\begin{matrix}
    A \\
    B 
\end{matrix}
\Big) = 
\Big(
\begin{matrix}
v_0^d - v_0^p - \gamma^p \, (v_0^p-V_0) \, \sinh(L_p) \\
- \gamma^p \, (v_0^p-V_0) \, \cosh(L_p)
\end{matrix}
\Big)
\end{equation}

And we solved this equation with the =solve_linear_system_LU= method of =sympy=

The coefficients $A$ and $B$ are given by:
\begin{equation}
A=\frac{\alpha}{\beta} \qquad \qquad B=\frac{\gamma}{\delta}
\end{equation}

where:

\begin{equation}
\begin{split}
& \alpha = V_{0} \gamma^{P} \lambda^{D} \cosh{\left (L_{p} \right )}
\cosh{\left (L - L_{p} \right )} + V_{0} \gamma^{P} \lambda^{P}
\sinh{\left (L_{p} \right )} \sinh{\left (L - L_{p} \right )} \\
& \quad - \gamma^{P} \lambda^{D} v^{d}_{0} \cosh{\left (L_{p} \right )}
\cosh{\left (L - L_{p} \right )} - \gamma^{P} \lambda^{P} v^{d}_{0}
\sinh{\left (L_{p} \right )} \sinh{\left (L - L_{p} \right )} \\
& \quad - \lambda^{P} v^{d}_{0} \sinh{\left (L - L_{p} \right )}
 + \lambda^{P} v^{p}_{0} \sinh{\left (L - L_{p} \right )} \\
& \beta = \gamma^{P} \lambda^{D} \cosh{\left (L_{p} \right )}
\cosh{\left (L - L_{p} \right )} + \gamma^{P} \lambda^{P} \sinh{\left
(L_{p} \right )} \sinh{\left (L - L_{p} \right )} + \\
& \quad \lambda^{D} \sinh{\left (L_{p} \right )} \cosh{\left (L - L_{p} \right )}
 + \lambda^{P} \sinh{\left (L - L_{p} \right )} \cosh{\left (L_{p} \right
)} \\
& \gamma = \lambda^{D} \big( V_{0} \gamma^{P} + \gamma^{P} v^{d}_{0}
\cosh{\left (L_{p} \right )} - \gamma^{P} v^{d}_{0} \\
& \quad  - \gamma^{P}
v^{p}_{0} \cosh{\left (L_{p} \right )} + v^{d}_{0} \sinh{\left (L_{p}
\right )} - v^{p}_{0} \sinh{\left (L_{p} \right )} \big) \\
& \delta = \gamma^{P}
\lambda^{D} \cosh{\left (L_{p} \right )} \cosh{\left (L - L_{p} \right
)} + \gamma^{P} \lambda^{P} \sinh{\left (L_{p} \right )} \sinh{\left
(L - L_{p} \right )}  \\
& \quad + \lambda^{D} \sinh{\left (L_{p} \right )}
\cosh{\left (L - L_{p} \right )}  + \lambda^{P} \sinh{\left (L - L_{p}
\right )} \cosh{\left (L_{p} \right )}
\end{split}
\end{equation}


* Derivation of the post-synaptic membrane potential event

For the PSP events we need to solve:

\begin{equation}
\left\{
\begin{split}
& \frac{\partial^2 \hat{\delta v}}{\partial X^2} =
\big( \alpha_f^p + (\alpha_f^d-\alpha_f^p) 
\mathcal{H}(X-L_p) \big)^2 \, 
\hat{\delta v}  \\
& \frac{\partial \hat{\delta v}}{\partial X}_{|X=0} = 
 \gamma_f^p \,  \hat{\delta v}(0,f) \\
&  \hat{\delta v}(X_{src}^-,f) = \hat{\delta v}(X_{src}^+,f) \\
& \frac{\partial \hat{\delta v}}{\partial X}_{X_{src}^-} 
= \frac{\partial \hat{\delta v}}{\partial X}_{X_{src}^+} 
- \big(\mu_v(X_{src})-E_{rev}\big) \, \big( r_f^p + (r_f^d-r_f^p) \mathcal{H}(X_{src}-L_p) \big) \, \hat{g(f)} \\
& \hat{\delta v}(L_p^-,f) = \hat{\delta v}(L_p^+,f) \\
& \frac{\partial \hat{\delta v}}{\partial X}_{L_p^-} 
= \frac{\lambda^p}{\lambda^d} \, 
\frac{\partial \hat{\delta v}}{\partial X}_{L_p^+} \\
& \frac{\partial \hat{\delta v}}{\partial X}_{X=L} = 0
\end{split}
\right.
\end{equation}



\begin{equation}
& A_f(X_src)=\frac{I_{f} r^{P}_{f} \left(- \alpha^{D}_{f} \lambda^{P} \cosh{\left (L \alpha^{D}_{f} - L_{p} \alpha^{D}_{f} - L_{p} \alpha^{P}_{f} + X_{s} \alpha^{P}_{f} \right )} + \alpha^{D}_{f} \lambda^{P} \cosh{\left (L \alpha^{D}_{f} - L_{p} \alpha^{D}_{f} + L_{p} \alpha^{P}_{f} - X_{s} \alpha^{P}_{f} \right )} + \alpha^{P}_{f} \lambda^{D} \cosh{\left (L \alpha^{D}_{f} - L_{p} \alpha^{P}_{f} - X_{s} \alpha^{D}_{f} + X_{s} \alpha^{P}_{f} \right )} + \alpha^{P}_{f} \lambda^{D} \cosh{\left (L \alpha^{D}_{f} + L_{p} \alpha^{P}_{f} - X_{s} \alpha^{D}_{f} - X_{s} \alpha^{P}_{f} \right )}\right)}{\alpha^{P}_{f} \left(- \alpha^{D}_{f} \gamma^{P}_{f} \lambda^{P} \cosh{\left (- L \alpha^{D}_{f} + L_{p} \alpha^{D}_{f} + L_{p} \alpha^{P}_{f} \right )} + \alpha^{D}_{f} \gamma^{P}_{f} \lambda^{P} \cosh{\left (L \alpha^{D}_{f} - L_{p} \alpha^{D}_{f} + L_{p} \alpha^{P}_{f} \right )} - \alpha^{D}_{f} \lambda^{P} \sinh{\left (- L \alpha^{D}_{f} + L_{p} \alpha^{D}_{f} + L_{p} \alpha^{P}_{f} \right )} + \alpha^{D}_{f} \lambda^{P} \sinh{\left (L \alpha^{D}_{f} - L_{p} \alpha^{D}_{f} + L_{p} \alpha^{P}_{f} \right )} + \alpha^{P}_{f} \gamma^{P}_{f} \lambda^{D} \cosh{\left (- L \alpha^{D}_{f} + L_{p} \alpha^{P}_{f} + X_{s} \alpha^{D}_{f} \right )} + \alpha^{P}_{f} \gamma^{P}_{f} \lambda^{D} \cosh{\left (L \alpha^{D}_{f} + L_{p} \alpha^{P}_{f} - X_{s} \alpha^{D}_{f} \right )} + \alpha^{P}_{f} \lambda^{D} \sinh{\left (- L \alpha^{D}_{f} + L_{p} \alpha^{P}_{f} + X_{s} \alpha^{D}_{f} \right )} + \alpha^{P}_{f} \lambda^{D} \sinh{\left (L \alpha^{D}_{f} + L_{p} \alpha^{P}_{f} - X_{s} \alpha^{D}_{f} \right )}\right)}
& B_f(X_src)=\frac{I_{f} \lambda^{D} r^{P}_{f} \left(\gamma^{P}_{f} \sinh{\left (- L \alpha^{D}_{f} + X_{s} \alpha^{D}_{f} + X_{s} \alpha^{P}_{f} \right )} + \gamma^{P}_{f} \sinh{\left (L \alpha^{D}_{f} - X_{s} \alpha^{D}_{f} + X_{s} \alpha^{P}_{f} \right )} + \cosh{\left (- L \alpha^{D}_{f} + X_{s} \alpha^{D}_{f} + X_{s} \alpha^{P}_{f} \right )} + \cosh{\left (L \alpha^{D}_{f} - X_{s} \alpha^{D}_{f} + X_{s} \alpha^{P}_{f} \right )}\right)}{- \alpha^{D}_{f} \gamma^{P}_{f} \lambda^{P} \cosh{\left (- L \alpha^{D}_{f} + L_{p} \alpha^{D}_{f} + L_{p} \alpha^{P}_{f} \right )} + \alpha^{D}_{f} \gamma^{P}_{f} \lambda^{P} \cosh{\left (L \alpha^{D}_{f} - L_{p} \alpha^{D}_{f} + L_{p} \alpha^{P}_{f} \right )} - \alpha^{D}_{f} \lambda^{P} \sinh{\left (- L \alpha^{D}_{f} + L_{p} \alpha^{D}_{f} + L_{p} \alpha^{P}_{f} \right )} + \alpha^{D}_{f} \lambda^{P} \sinh{\left (L \alpha^{D}_{f} - L_{p} \alpha^{D}_{f} + L_{p} \alpha^{P}_{f} \right )} + \alpha^{P}_{f} \gamma^{P}_{f} \lambda^{D} \cosh{\left (- L \alpha^{D}_{f} + L_{p} \alpha^{P}_{f} + X_{s} \alpha^{D}_{f} \right )} + \alpha^{P}_{f} \gamma^{P}_{f} \lambda^{D} \cosh{\left (L \alpha^{D}_{f} + L_{p} \alpha^{P}_{f} - X_{s} \alpha^{D}_{f} \right )} + \alpha^{P}_{f} \lambda^{D} \sinh{\left (- L \alpha^{D}_{f} + L_{p} \alpha^{P}_{f} + X_{s} \alpha^{D}_{f} \right )} + \alpha^{P}_{f} \lambda^{D} \sinh{\left (L \alpha^{D}_{f} + L_{p} \alpha^{P}_{f} - X_{s} \alpha^{D}_{f} \right )}}
& C_f(X_src)=\frac{I_{f} \alpha^{D}_{f} \lambda^{P} r^{P}_{f} \left(\gamma^{P}_{f} \cosh{\left (- L \alpha^{D}_{f} + L_{p} \alpha^{D}_{f} + X_{s} \alpha^{P}_{f} \right )} - \gamma^{P}_{f} \cosh{\left (L \alpha^{D}_{f} - L_{p} \alpha^{D}_{f} + X_{s} \alpha^{P}_{f} \right )} + \sinh{\left (- L \alpha^{D}_{f} + L_{p} \alpha^{D}_{f} + X_{s} \alpha^{P}_{f} \right )} - \sinh{\left (L \alpha^{D}_{f} - L_{p} \alpha^{D}_{f} + X_{s} \alpha^{P}_{f} \right )}\right)}{\alpha^{P}_{f} \left(- \alpha^{D}_{f} \gamma^{P}_{f} \lambda^{P} \cosh{\left (- L \alpha^{D}_{f} + L_{p} \alpha^{D}_{f} + L_{p} \alpha^{P}_{f} \right )} + \alpha^{D}_{f} \gamma^{P}_{f} \lambda^{P} \cosh{\left (L \alpha^{D}_{f} - L_{p} \alpha^{D}_{f} + L_{p} \alpha^{P}_{f} \right )} - \alpha^{D}_{f} \lambda^{P} \sinh{\left (- L \alpha^{D}_{f} + L_{p} \alpha^{D}_{f} + L_{p} \alpha^{P}_{f} \right )} + \alpha^{D}_{f} \lambda^{P} \sinh{\left (L \alpha^{D}_{f} - L_{p} \alpha^{D}_{f} + L_{p} \alpha^{P}_{f} \right )} + \alpha^{P}_{f} \gamma^{P}_{f} \lambda^{D} \cosh{\left (- L \alpha^{D}_{f} + L_{p} \alpha^{P}_{f} + X_{s} \alpha^{D}_{f} \right )} + \alpha^{P}_{f} \gamma^{P}_{f} \lambda^{D} \cosh{\left (L \alpha^{D}_{f} + L_{p} \alpha^{P}_{f} - X_{s} \alpha^{D}_{f} \right )} + \alpha^{P}_{f} \lambda^{D} \sinh{\left (- L \alpha^{D}_{f} + L_{p} \alpha^{P}_{f} + X_{s} \alpha^{D}_{f} \right )} + \alpha^{P}_{f} \lambda^{D} \sinh{\left (L \alpha^{D}_{f} + L_{p} \alpha^{P}_{f} - X_{s} \alpha^{D}_{f} \right )}\right)}
& D_f(X_src)=\frac{2 I_{f} \lambda^{D} r^{P}_{f} \left(\gamma^{P}_{f} \sinh{\left (X_{s} \alpha^{P}_{f} \right )} + \cosh{\left (X_{s} \alpha^{P}_{f} \right )}\right)}{- \alpha^{D}_{f} \gamma^{P}_{f} \lambda^{P} \cosh{\left (- L \alpha^{D}_{f} + L_{p} \alpha^{D}_{f} + L_{p} \alpha^{P}_{f} \right )} + \alpha^{D}_{f} \gamma^{P}_{f} \lambda^{P} \cosh{\left (L \alpha^{D}_{f} - L_{p} \alpha^{D}_{f} + L_{p} \alpha^{P}_{f} \right )} - \alpha^{D}_{f} \lambda^{P} \sinh{\left (- L \alpha^{D}_{f} + L_{p} \alpha^{D}_{f} + L_{p} \alpha^{P}_{f} \right )} + \alpha^{D}_{f} \lambda^{P} \sinh{\left (L \alpha^{D}_{f} - L_{p} \alpha^{D}_{f} + L_{p} \alpha^{P}_{f} \right )} + \alpha^{P}_{f} \gamma^{P}_{f} \lambda^{D} \cosh{\left (- L \alpha^{D}_{f} + L_{p} \alpha^{P}_{f} + X_{s} \alpha^{D}_{f} \right )} + \alpha^{P}_{f} \gamma^{P}_{f} \lambda^{D} \cosh{\left (L \alpha^{D}_{f} + L_{p} \alpha^{P}_{f} - X_{s} \alpha^{D}_{f} \right )} + \alpha^{P}_{f} \lambda^{D} \sinh{\left (- L \alpha^{D}_{f} + L_{p} \alpha^{P}_{f} + X_{s} \alpha^{D}_{f} \right )} + \alpha^{P}_{f} \lambda^{D} \sinh{\left (L \alpha^{D}_{f} + L_{p} \alpha^{P}_{f} - X_{s} \alpha^{D}_{f} \right )}}
\end{equation}


